Verified derivation with substitution. Some missing cases. Changed the signature of tryDeriveJustification

ModularEngine/src/LogicEngine.FStar/coredkal2.fst
@@ -95,7 +95,7 @@ type entails :: substrate => infostrate => varDecl => term => P =
     -> entails S K G (ForallT v i)
     -> types G u v.typ
     -> entails S K G i'
-
+ 
   | Entails_And_Intro : 
        S:substrate -> K:infostrate -> G:varDecl
     -> ilist:list term -> pref:prefix
@@ -109,12 +109,24 @@ type entails :: substrate => infostrate => varDecl => term => P =
     -> entails S K G (WithPrefix pref j)
     -> entails S K G (WithPrefix pref (App AndInfon [i;j]))
 
-  | Entails_And_Elim : 
+  | Entails_And_Elim : (* + well-typedness condition? *)
        S:substrate -> K:infostrate -> G:varDecl
     -> ilist:list term -> i:term{In i ilist} -> pref:prefix
     -> entails S K G (WithPrefix pref (App AndInfon ilist))
     -> entails S K G (WithPrefix pref i)
-
+    
+  | Entails_And_Elim1 : 
+       S:substrate -> K:infostrate -> G:varDecl
+    -> i1:term -> i2:term -> pref:prefix
+    -> entails S K G (WithPrefix pref (App AndInfon [i1; i2]))
+    -> entails S K G (WithPrefix pref i1)
+    
+  | Entails_And_Elim2 : 
+       S:substrate -> K:infostrate -> G:varDecl
+    -> i1:term -> i2:term -> pref:prefix
+    -> entails S K G (WithPrefix pref (App AndInfon [i1; i2]))
+    -> entails S K G (WithPrefix pref i2)
+    
   | Entails_W_Imp_Intro : 
        S:substrate -> K:infostrate -> G:varDecl
     -> i:term -> j:term -> pref:prefix
@@ -151,18 +163,33 @@ type result :: _ =
         (goal':term{Subst goal s3 goal'} * pref':prefix{SubstList pref s3 pref'} * entails s k g (WithPrefix pref' goal')))
         (* (goal':term{Subst goal s4 goal'} * pref':prefix{SubstList pref s4 pref'} * entails s k g (WithPrefix pref' goal'))) *)
 
+val last : pref:prefix 
+        -> res:option (term * prefix) {
+		     forall (p:term) (tl2:prefix) (t:term).
+			   (res = (Some (p, tl2)))
+			     => (WithPrefix [p] (WithPrefix tl2 t)) = (WithPrefix pref t)}
+(*
+let rec last pref = 
+  match pref with
+    | [] -> None
+	(*| hd::[] -> Some(hd, []) *) (* Rk: this line raises an error *)
+	| hd::tl -> match last tl with
+	              | None -> (* tl = [] *) Some(hd, [])
+				  | Some((p, tl2)) -> Some(p, hd::tl2)
+*) 
+		
 val doDerive:   S:substrate 
              -> K:infostrate 
              -> G:varDecl
              -> U:varDecl             (* Variables available for unification in goal *)
-     	     -> s1:substitution
+             -> s1:substitution
              -> pref:prefix 
              -> goal:term
              -> option (s2:substitution{Extends s2 s1} *
                           (s3:substitution{Extends s3 s2} ->  (goal':term{Subst goal s3 goal'} *
                                                                  pref':prefix{SubstList pref s3 pref'} *
                                                                  entails S K G (WithPrefix pref' goal'))))
-
+																 
 val unify: u:varDecl 
         -> s1:substitution
         -> i:term    
@@ -172,79 +199,223 @@ val unify: u:varDecl
      informally, only variables in u are available for unification.
 *)
 
+(* tries to prove (withPrefix pref goal) using (infon);
+   but really what we will eventually prove is
+   (withPrefix pref_infon (withPrefix pref goal))
+   and we really know (withPrefix pref_infon infon)
+*)
 val tryDerive:  S:substrate 
              -> K:infostrate 
              -> G:varDecl
              -> U:varDecl             (* Variables available for unification in goal *)
-     	     -> s1:substitution
+             -> s1:substitution
              -> pref:prefix 
-             -> i:term{In i K}
              -> goal:term
+             -> pref_infon:prefix (* suff in original implementation *)
+             -> infon:term
+             -> mkpf_infon:(s4:substitution{Extends s4 s1}
+                             -> (infon':term{Subst infon s4 infon'} *
+                                 pref_infon':prefix{SubstList pref_infon s4 pref_infon'} *
+                                 entails S K G (WithPrefix pref_infon' infon')))
              -> option (s2:substitution{Extends s2 s1} *
-                          (s3:substitution{Extends s3 s2} -> (goal':term{Subst goal s3 goal'} *
-                                                                pref':prefix{SubstList pref s3 pref'} *
-                                                                entails S K G (WithPrefix pref' goal'))))
-let tryDerive s k g u s1 pref i goal = 
-  let pref_goal = withPrefix pref goal in
-    match unify u s1 i pref_goal with 
+                          (s3:substitution{Extends s3 s2} 
+                             -> (goal':term{Subst goal s3 goal'} *
+                                 pref':prefix{SubstList pref s3 pref'} *
+                                 entails S K G (WithPrefix pref' goal'))))
+
+let rec tryDerive s k g u s1 pref goal pref_infon infon mkpf_infon = 
+  match infon with
+  | App AndInfon [infon1; infon2] ->
+      let mkpf_infon1 (s4:substitution{Extends s4 s1}) =
+        let (infon', pref_infon', pf_infon') = mkpf_infon s4 in
+        let infon1' = subst infon1 s4 in (* inefficient, should grab the one from infon' *)
+        let infon2' = subst infon2 s4 in
+        if infon' = App AndInfon [infon1'; infon2']
+        then ((infon1', pref_infon', 
+               Entails_And_Elim1 s k g infon1' infon2' pref_infon' pf_infon') :                             
+                (infon1':term{Subst infon1 s4 infon1'} *
+                 pref_infon':prefix{SubstList pref_infon s4 pref_infon'} *
+                 entails s k g (WithPrefix pref_infon' infon1')))
+        else raise "impos" in (* not completely true: nondeterminism of substitution *)
+      (match tryDerive s k g u s1 pref goal pref_infon infon1 mkpf_infon1 with
+         | Some res -> Some res
+         | None -> 
+            let mkpf_infon2 (s4:substitution{Extends s4 s1}) =
+              let (infon', pref_infon', pf_infon') = mkpf_infon s4 in
+              let infon1' = subst infon1 s4 in
+              let infon2' = subst infon2 s4 in
+              if infon' = App AndInfon [infon1'; infon2']
+              then ((infon2', pref_infon', 
+                     Entails_And_Elim2 s k g infon1' infon2' pref_infon' pf_infon') :                             
+                      (infon2':term{Subst infon2 s4 infon2'} *
+                       pref_infon':prefix{SubstList pref_infon s4 pref_infon'} *
+                       entails s k g (WithPrefix pref_infon' infon2')))
+              else raise "impos" in 
+            tryDerive s k g u s1 pref goal pref_infon infon1 mkpf_infon1) 
+                     
+  | App ImpliesInfon [i; j] ->
+      (match doDerive s k g u s1 pref_infon i with (* for now, []; later change it, cf. suff *)
+         | None -> None
+         | Some((s2, mkpf_i)) ->
+             let mkpf_j (s4:substitution{Extends s4 s2}) =
+               let (i', pref_i', pf_i') = mkpf_i s4 in
+               let (infon', pref_infon', pf_infon') = mkpf_infon s4 in
+               let j' = subst j s4 in
+               if ((infon' = App ImpliesInfon [i'; j']) && (pref_i' = pref_infon'))
+               then ((j', pref_infon',
+                      Entails_Imp_Elim s k g i' j' pref_infon' pf_i' pf_infon') :
+                       (j':term{Subst j s4 j'} *
+                        pref_infon':prefix{SubstList pref_infon s4 pref_infon'} *
+                        entails s k g (WithPrefix pref_infon' j')))
+               else raise "impos" in None
+             (* ?? *) (*tryDerive s k g u s2 pref goal pref_infon j mkpf_j*))
+(*			 
+  | (App SaidInfon [p2; i]) (*when (last pref <> None)*) -> (* TODO: parsing *)
+      (match last pref with
+	     | None -> raise "impos" (* could assert false *)
+		 | Some((p1, pref1)) ->
+		     match unify u s1 p2(*infon*) p1(*goal*) with
+			   | None -> None
+			   | Some s2 ->
+			       (*let continuation (s3:substitution{Extends s3 s2}) =/*)
+				     let p2' = subst p2 s2 in
+				     if (p2':term) = p1
+					 then 
+					   tryDerive s k g u s2 pref1 goal (p2'::pref_infon) i mkpf_infon
+					 else raise "bad substitution"
+				   (*in Some(s2, continuation) *))
+*)	
+
+	
+(*
+  | _ -> let pref_goal = withPrefix pref goal in
+    match unify u s1 infon pref_goal with 
       | None -> None
       | Some s2 -> 
           let continuation (s3:substitution{Extends s3 s2}) = 
             let goal' = subst goal s3 in  (* Subst goal s3 goal' *)
             let pref' = substList pref s3 in  (* SubstList pref s3 pref' *)
             let pref_goal' = withPrefix pref' goal' in  (* pref_goal'= (WithPrefix pref' goal') *)
-              if (pref_goal':term) = i then 
-                match checkWF s k g with 
-                  | Some pf_wf -> 
-                      let pf = Entails_Hyp_Knowledge s k g i pf_wf in 
-                        ((goal', pref', pf) : 
-                           (goal':term{Subst goal s3 goal'} *
-                              pref':prefix{SubstList pref s3 pref'} *
-                              entails s k g (WithPrefix pref' goal')))
-                  | None -> raise "ill-formed environment"
+              if (pref_goal':term) = infon then 
+                ((goal', pref', pf_infon) : 
+                   (goal':term{Subst goal s3 goal'} *
+                    pref':prefix{SubstList pref s3 pref'} *
+                    entails s k g (WithPrefix pref' goal')))
               else raise "bad substitution" in 
             Some (s2, continuation)
+*)
+                
 
 (* result S K G s3 pref goal) *)
-let rec doDerive s k g u s1 pref goal = 
-  match map_one k (fun (i:term{In i k}) -> tryDerive s k g u s1 pref i goal) with (* should this be done last? *)
-    | Some result -> Some result
-    | None -> 
-        match goal with 
-          | App AndInfon [goal_i; goal_j] -> 
-              (match doDerive s k g u s1 pref goal_i with 
-                 | None -> None
-                 | Some((s2, mkpf_i)) -> 
-                     match doDerive s k g u s2 pref goal_j with 
-                       | None -> None
-                       | Some((s3, mkpf_j)) -> 
-                           let continuation (s4:substitution{Extends s4 s3}) = 
-                             let goal_i', pref_i', pf_i' = mkpf_i s4 in (* from lemma: Extends s4 s2 *) (* pf_i': entails s k g (WithPrefix pref_i' goal_i') *) 
-                             let goal_j', pref_j', pf_j' = mkpf_j s4 in (* Extends s4 s3, directly *) (* pf_j': entails s k g (WithPrefix pref_j' goal_j') *)
-                               if (pref_i'=pref_j') (* we know: Subst pref s4 pref_i' and  Subst pref s4 pref_j'; but not pref_i'=pref_j' *)
-                               then
-                                 let pf_and = Entails_And_Intro2 s k g goal_i' goal_j' pref_i' pf_i' pf_j' in
-                                 let goal' = App AndInfon [goal_i'; goal_j'] in  (* pf_and: Entails s k g goal'*)
-                                   ((goal', pref_i', pf_and)
-                                      :(goal':term{Subst goal s4 goal'} * pref':prefix{SubstList pref s4 pref'} * entails s k g (WithPrefix pref' goal')))
-                               else raise "bad substitution" in 
-                             Some (s3, continuation))
-                
-          | App SaidInfon [p;j] ->
-              (match doDerive s k g u s1 (p::pref) j with
-                 | Some ((s2, mkpf_j)) ->  (* s2:substitution{Extends s2 s1} * (s3:subst{Extends s3 s2} -> (goal_j':term{Subst goal_j s3 goal_j'} *
-                                              pref_j':prefix{SubstList (p::pref) s3 pref'} *
-                                              entails s k g (WithPrefix pref_j' goal_j'))) *)
-                     let continuation (s3:substitution{Extends s3 s2}) =
-                       let goal_j', pref_j', pf_j' = mkpf_j s3 in (* SubstList (p::pref) s3 pref_j'; we should prove that pref_j' = p'::pref' where (Subst p s3 p') *)
-                         match pref_j' with
-                           | p'::pref' -> (* should prove that (Subst p s3 p') *)
-                               let goal' = App SaidInfon [p'; goal_j'] in
-                                 ((goal', pref', pf_j')
-                                    : (goal':term{Subst goal s3 goal'} * pref':prefix{SubstList pref s3 pref'} * entails s k g (WithPrefix pref' goal')))
-                           | [] -> raise "impos" in (* prove that this case is unreachable by asserting false *) 
-                       Some (s2, continuation))
+and doDerive s k g u s1 pref goal = 
+  match goal with
+  | App EmptyInfon [] -> 
+      let continuation (s2:substitution{Extends s2 s1}) =
+        let pref' = substList pref s2 in
+        match checkWF s k g, 
+              doType g (WithPrefix pref' (App EmptyInfon [])) with 
+          | Some pf_wf, Some((Infon, pf_typ)) ->
+              ((goal, pref', Entails_Emp s k g pref' pf_wf pf_typ) :
+                 (goal':term{Subst goal s2 goal'} *
+                    pref':prefix{SubstList pref s2 pref'} *
+                    entails s k g (WithPrefix pref' goal')))
+          | None, _ -> raise "ill-formed environment"
+          | _, None -> raise "ill-typed term"
+      in Some(s1, continuation) 
 
-          | _ -> None (* todo *)
-              
-              
+  | App AndInfon [goal_i; goal_j] -> 
+      (match doDerive s k g u s1 pref goal_i with 
+         | None -> None
+         | Some((s2, mkpf_i)) -> 
+             match doDerive s k g u s2 pref goal_j with 
+               | None -> None
+               | Some((s3, mkpf_j)) -> 
+                   let continuation (s4:substitution{Extends s4 s3}) = 
+                     let goal_i', pref_i', pf_i' = mkpf_i s4 in (* from lemma: Extends s4 s2 *) (* pf_i': entails s k g (WithPrefix pref_i' goal_i') *) 
+                     let goal_j', pref_j', pf_j' = mkpf_j s4 in (* Extends s4 s3, directly *) (* pf_j': entails s k g (WithPrefix pref_j' goal_j') *)
+                       if (pref_i'=pref_j') (* we know: Subst pref s4 pref_i' and  Subst pref s4 pref_j'; but not pref_i'=pref_j' *)
+                       then
+                         let pf_and = Entails_And_Intro2 s k g
+                                        goal_i' goal_j' pref_i' pf_i' pf_j' in
+                         let goal' = App AndInfon [goal_i'; goal_j'] in  (* pf_and: Entails s k g goal'*)
+                           ((goal', pref_i', pf_and)
+                              :(goal':term{Subst goal s4 goal'} *
+                                pref':prefix{SubstList pref s4 pref'} *
+                                entails s k g (WithPrefix pref' goal')))
+                       else raise "bad substitution" in 
+                     Some (s3, continuation))
+(*  
+  | App AsInfon [SubstrateQueryTerm q] ->
+      (match pref with
+         | [] ->
+            (match check_substrate s q with
+               | false -> None
+               | true ->
+                  let continuation (s2:substitution{Extends s2 s1}) =
+                     match checkWF s k g, subst goal s2 with
+                       | None, _ -> raise "ill-formed environment"
+                       | Some pf_wf, App AsInfon [SubstrateQueryTerm q'] ->
+                           let pf = Entails_Hyp_Substrate s k g q pf_wf in
+                           let goal' = subst goal s2 in
+                           let pref' = substList pref s2 in
+                             ((goal', pref', pf) 
+                                 :(goal':term{Subst goal s2 goal'} *
+                                   pref':prefix{SubstList pref s2 pref'} *
+                                   entails s k g (WithPrefix pref' goal')))
+					   | _ -> raise "impos"
+                   in
+                     Some(s1, continuation) )
+         | _ -> raise "asInfon(...) under prefix")
+*)  
+  | App ImpliesInfon [goal_i; goal_j] ->
+      (match doDerive s k g u s1 pref goal_j with
+         | None -> None
+         | Some((s2, mkpf_j)) ->
+             let continuation (s3:substitution{Extends s3 s2}) =
+               let goal_j', pref_j', pf_j' = mkpf_j s3 in
+               let goal_i' = subst goal_i s3 in
+               match doType g goal_i' with
+                 | Some((Infon, pf_typ)) ->
+                     let pf_imp = Entails_W_Imp_Intro s k g 
+                                goal_i' goal_j' pref_j' pf_j' pf_typ in
+                     let goal' = App ImpliesInfon [goal_i'; goal_j'] in
+                       ((goal', pref_j', pf_imp)
+                          : (goal':term{Subst goal s3 goal'} *
+                             pref':prefix{SubstList pref s3 pref'} *
+                             entails s k g (WithPrefix pref' goal')))
+                 | None -> raise "ill-typed term" in
+             Some (s2, continuation))
+             
+               
+  | App SaidInfon [p;j] ->
+      (match doDerive s k g u s1 (p::pref) j with
+         | Some ((s2, mkpf_j)) ->  (* s2:substitution{Extends s2 s1} * (s3:subst{Extends s3 s2} -> (goal_j':term{Subst goal_j s3 goal_j'} *
+                                      pref_j':prefix{SubstList (p::pref) s3 pref'} *
+                                      entails s k g (WithPrefix pref_j' goal_j'))) *)
+             let continuation (s3:substitution{Extends s3 s2}) =
+               let goal_j', pref_j', pf_j' = mkpf_j s3 in (* SubstList (p::pref) s3 pref_j'; we should prove that pref_j' = p'::pref' where (Subst p s3 p') *)
+                 match pref_j' with
+                   | p'::pref' -> (* should prove that (Subst p s3 p') *)
+                       let goal' = App SaidInfon [p'; goal_j'] in
+                         ((goal', pref', pf_j')
+                            : (goal':term{Subst goal s3 goal'} * pref':prefix{SubstList pref s3 pref'} * entails s k g (WithPrefix pref' goal')))
+                   | [] -> raise "impos" in (* prove that this case is unreachable by asserting false *) 
+               Some (s2, continuation))
+(*
+  | _ -> 
+      let call_tryDerive (infon:term{In infon k}) =
+        let mkpf_infon (s2:substitution{Extends s2 s1}) : entails s k g infon =
+           (match checkWF s k g with
+              | None -> raise "ill-formed environment"
+              | Some pf_wf -> (* this is P-kinded, I don't get it *)	    
+	              let infon' = subst infon s2 in
+		 	  	  if infon = infon'
+			      then (infon', [],
+				        Entails_Hyp_Knowledge s k g infon pf_wf)
+			      else raise "not a closed infon in infostrate") in
+        tryDerive s k g u s1 pref goal [] infon mkpf_infon in
+      match map_one k call_tryDerive with (* should this be done last? *)
+        | Some result -> Some result
+        | None -> None
+*)
+          
